src/Prototype/Locality.v
@@ -1,14 +1,40 @@
 Require Import Bool List String Peano_dec.
-Require Import FMap Language Transaction.
+Require Import FMap Language Transaction Monotone.
 
-Section History.
-  Variables MsgT StateT: Type.
+Section Facts.
+  Context {MsgT ValT StateT: Type}.
+  Hypothesis (msgT_dec : forall m1 m2 : MsgT, {m1 = m2} + {m1 <> m2}).
+  Hypothesis (valT_dec : forall v1 v2 : ValT, {v1 = v2} + {v1 <> v2}).
 
-  Local Notation MsgId := (MsgId MsgT).
-  Local Notation Object := (Object MsgT StateT).
-  Local Notation System := (System MsgT StateT).
+  Local Notation System := (System MsgT ValT StateT).
 
-  (* Inductive TrsSeq: list MsgId -> Prop := *)
+  Theorem linear_sequential_compositional:
+    forall sys: System,
+      MonotoneSys msgT_dec sys ->
+      Forall (fun obj => SequentialSys msgT_dec valT_dec (obj :: nil)) sys ->
+      Linear msgT_dec valT_dec sys.
+  Proof.
+  Admitted.
 
-End History.
+  Corollary disjoint_linear:
+    forall sys: System,
+      MonotoneSys msgT_dec sys ->
+      Forall (LocallyDisjoint msgT_dec) sys ->
+      Linear msgT_dec valT_dec sys.
+  Proof.
+    intros; apply linear_sequential_compositional; auto.
+    apply Forall_impl with (P:= LocallyDisjoint msgT_dec); auto.
+    intros; apply locally_disjoint_sequential; auto.
+  Qed.
+
+  Theorem prioritized_interf_linear_compositional:
+    forall sys: System,
+      MonotoneSys msgT_dec sys ->
+      Forall (fun obj => Linear msgT_dec valT_dec (obj :: nil)) sys ->
+      Forall (PInterfering msgT_dec) sys ->
+      Linear msgT_dec valT_dec sys.
+  Proof.
+  Admitted.
+
+End Facts.
 
